bound/UpperBound_AExtra.v
@@ -1,18 +1,72 @@
- Require Import CoqlibC Maps.
+Require Import CoqlibC MapsC.
 Require Import ASTC Integers Floats Values MemoryC Events Globalenvs Smallstep.
 Require Import Locations Stacklayout Conventions Linking.
 Require Export Csem Cop Ctypes Ctyping Csyntax Cexec.
 Require Import Simulation Memory ValuesC.
 Require Import Skeleton ModSem Mod sflib.
-Require Import CtypesC CsemC Sem Syntax LinkingC Program.
+Require Import CtypesC CsemC Sem Syntax LinkingC Program SemProps.
 Require Import Equality.
 Require Import CtypingC.
-Require Import UpperBound_A.
-Require Import UpperBound_A.
+(* Require Import UpperBound_A. *)
 
 Set Implicit Arguments.
 
+Ltac Eq :=
+  match goal with
+  | [ H1: ?a = ?b, H2: ?a = ?c |- _ ] =>
+    rewrite H1 in H2; inv H2; Eq
+  | [ H1: ?a m= ?b, H2: ?a m= ?c |- _ ] =>
+    rewrite H1 in H2; inv H2; Eq
+  | _ => idtac
+  end.
 
+Fixpoint app_cont (k0 k1: cont) {struct k0}: cont :=
+  match k0 with
+  | Kstop => k1
+  | Kdo k => Kdo (app_cont k k1)
+  | Kseq s k => Kseq s (app_cont k k1)
+  | Kifthenelse s1 s2 k => Kifthenelse s1 s2 (app_cont k k1)
+  | Kwhile1 e s k => Kwhile1 e s (app_cont k k1)
+  | Kwhile2 e s k => Kwhile2 e s (app_cont k k1)
+  | Kdowhile1 e s k => Kdowhile1 e s (app_cont k k1)
+  | Kdowhile2 e s k => Kdowhile2 e s (app_cont k k1)
+  | Kfor2 e s1 s2 k => Kfor2 e s1 s2 (app_cont k k1)
+  | Kfor3 e s1 s2 k => Kfor3 e s1 s2 (app_cont k k1)
+  | Kfor4 e s1 s2 k => Kfor4 e s1 s2 (app_cont k k1)
+  | Kswitch1 ls k =>  Kswitch1 ls (app_cont k k1)
+  | Kswitch2 k =>  Kswitch2 (app_cont k k1)
+  | Kreturn k => Kreturn (app_cont k k1)
+  | Kcall f e em ty k => Kcall f e em ty (app_cont k k1)
+  end
+.
+
+Lemma app_cont_stop_right
+      k0
+  :
+    <<EQ: app_cont k0 Kstop = k0>>
+.
+Proof.
+  ginduction k0; ii; ss; des; clarify; ss; r; f_equal; ss.
+Qed.
+
+Lemma app_cont_stop_left
+      k0
+  :
+    <<EQ: app_cont Kstop k0 = k0>>
+.
+Proof.
+  ginduction k0; ii; ss; des; clarify; ss; r; f_equal; ss.
+Qed.
+
+Lemma app_cont_kstop_inv
+      k0 k1
+      (APP: app_cont k0 k1 = Kstop)
+  :
+    k0 = Kstop /\ k1 = Kstop
+.
+Proof.
+  destruct k0; ss.
+Qed.
 
 Section SIM.
 
@@ -28,9 +82,195 @@ Section SIM.
   Notation " 'geof' cp" := (Build_genv (SkEnv.revive (SkEnv.project skenv_link cp.(CSk.of_program signature_of_function)) cp) cp.(prog_comp_env))
                            (at level 50, no associativity, only parsing).
   Let ge_cp_link: genv := geof cp_link.
+  Hypothesis WTPROGLINK: wt_program cp_link.
+  Hypothesis WTPROGS: forall cp (IN: In cp cps), wt_program cp.
+  (* Hypothesis WTSKS: forall cp (IN: In cp cps), Sk.wf cp.(CsemC.module). *)
 
-  Let sum_cont := sum_cont cps sk_link.
-  (* Variable cp_link cp0 cp1: Csyntax.program. *)
+  Definition is_focus (cp: Csyntax.program): Prop := In cp cps.
+  (* put k1 inside k0 (k1 is executed later) *)
+
+  Lemma link_sk_match
+    :
+      <<EQ: link_sk prog_src = link_sk prog_tgt>>
+  .
+  Proof.
+    subst_locals.
+    unfold link_sk.
+    rewrite ! map_app. ss.
+    symmetry.
+    eapply link_list_app_commut; eauto.
+
+    clear - FOCUS.
+    ginduction cps; ii; ss.
+    destruct l; ss.
+    { unfold link_list, link_list_aux in *. des_ifs. }
+    exploit link_list_cons_inv; eauto.
+    { ss. }
+    intro P; des.
+    exploit IHl; eauto. intro P; des.
+    exploit (@link_list_cons Sk.t); try apply P.
+    { instantiate (1:= CSk.of_program signature_of_function cp_link).
+      instantiate (1:= CSk.of_program signature_of_function a).
+      clear - HD.
+      Local Transparent Linker_prog Linker_program Linker_fundef Linker_types Linker_varinit
+            Linker_vardef Linker_def Linking.Linker_fundef.
+      ss.
+      rename a into p0. rename restl into p1. fold Csyntax.program in *.
+      (* Set Printing Implicit. *)
+      unfold link_program in *. des_ifs. ss.
+      clear - Heq.
+      unfold link_prog in *. ss. des_ifs_safe. bsimpl. des. des_sumbool.
+      des_ifs; cycle 1.
+      { exfalso. bsimpl. des; des_sumbool; ss.
+        rewrite PTree_Properties.for_all_false in *. rewrite PTree_Properties.for_all_correct in *.
+        des.
+        generalize (CSk.of_program_prog_defmap p0 signature_of_function x1). intro REL0.
+        generalize (CSk.of_program_prog_defmap p1 signature_of_function x1). intro REL1.
+        inv REL0; try by congruence.
+        rewrite <- H0 in *. clarify. exploit Heq1; eauto. intro CHK; des.
+        unfold link_prog_check in *. des_ifs_safe.
+        inv REL1. ss. rewrite <- H2 in *.
+        bsimpl. des; des_sumbool; ss; clarify.
+        clear - Heq2 CHK0 H1 H4.
+        des_ifs. inv H1; inv H4; ss.
+        - unfold CtypesC.CSk.match_fundef in *. des_ifs; ss; des_ifs. bsimpl; des; des_sumbool; clarify.
+        - des_ifs. inv H; inv H0; ss. unfold link_vardef in *. ss. des_ifs.
+      }
+      bsimpl. des. des_sumbool.
+      f_equal. unfold CSk.of_program. ss. f_equal.
+      unfold skdefs_of_gdefs. (* unfold prog_defmap. ss. *)
+      rewrite PTree_elements_map.
+      rewrite PTree_elements_map.
+      eapply PTree.elements_extensional. intro id. rewrite PTree.gcombine; ss.
+      rewrite ! PTree.gmap. rewrite PTree.gcombine; ss.
+      rename Heq2 into P. rename Heq1 into Q. clear - P Q.
+      unfold prog_defmap in *. ss.
+      rewrite ! prog_defmap_update_snd.
+      rewrite PTree_Properties.for_all_correct in *.
+      set ((PTree_Properties.of_list (prog_defs p0)) ! id) as x.
+      set ((PTree_Properties.of_list (prog_defs p1)) ! id) as y.
+      clear_tac.
+      destruct x eqn:Tx; ss. destruct y eqn:Ty; ss. unfold x in Tx. unfold y in Ty.
+      exploit Q; eauto. intro CHK. (* unfold link_prog_check, prog_defmap in CHK. *)
+      unfold option_map. des_ifs; ss; cycle 1.
+      - destruct g, g0; ss; unfold skdef_of_gdef, fundef_of_fundef in *; des_ifs; ss; des_ifs.
+        + unfold link_prog_check in CHK. unfold prog_defmap in *. unfold program_of_program in CHK. ss.
+          des_ifs_safe. bsimpl. des_safe. des_sumbool. des_ifs. bsimpl. des; ss; des_sumbool; clarify.
+        + unfold link_prog_check in CHK. unfold prog_defmap in *. unfold program_of_program in CHK. ss.
+          des_ifs_safe. bsimpl. des_safe.
+      - destruct g, g0; ss; unfold skdef_of_gdef, fundef_of_fundef in *; des_ifs; ss;
+          unfold fundef_of_fundef in *; des_ifs.
+        + destruct g; ss. unfold link_vardef in *. des_ifs. ss. bsimpl. des. rewrite eqb_true_iff in *.
+          f_equal. destruct gvar_info; ss. f_equal; ss. f_equal; ss. clarify.
+        + exfalso.
+          destruct v, v0; ss. unfold link_vardef in *. ss. des_ifs.
+    }
+    intro Q; des. ss.
+  Qed.
+
+  Let LINKTGT: link_sk prog_tgt = Some sk_link.
+  Proof.
+    rewrite link_sk_match in *. ss.
+  Qed.
+
+  Let INCL_LINKED: SkEnv.includes skenv_link (CSk.of_program signature_of_function cp_link).
+  Proof.
+    exploit link_includes. eapply LINKSRC.
+    subst prog_src. instantiate (1 := (module cp_link)).
+    apply in_or_app. ss. auto. ss. Qed.
+
+  Let INCL_FOCUS: forall pgm, is_focus pgm -> SkEnv.includes skenv_link (CSk.of_program signature_of_function pgm).
+  Proof.
+    i. exploit link_includes.
+    { eapply LINKTGT. }
+    { subst prog_tgt. instantiate (1 := (module pgm)).
+      rewrite in_app_iff in *. r in H. right. rewrite in_map_iff. esplits; et. }
+    i. ss.
+  Qed.
+
+  Lemma prog_defmap_func_same_rev
+        pgm id func
+        (FOC: is_focus pgm)
+        (DMAP: (prog_defmap pgm) ! id = Some (Gfun func)) (* (Internal func))) *)
+        (INTERNAL: negb (is_external_fd func) = true)
+    :
+      (prog_defmap cp_link) ! id = Some (Gfun func). (* (Internal func')). *)
+  Proof.
+    Local Transparent Linker_program. ss.
+    unfold link_program in *. des_ifs.
+    Local Transparent Linker_prog. ss.
+
+    r in FOC.
+    exploit link_list_linkorder; et. intro ORD. r in ORD. rewrite Forall_forall in ORD.
+    exploit ORD; eauto. intro ORD0.
+    Local Transparent Linker_program.
+    ss.
+    rr in ORD0. des.
+    hexploit (@prog_defmap_linkorder (Ctypes.fundef function) type); eauto. intro P; des. inv P0.
+    inv H0; ss.
+  Qed.
+
+  Inductive sum_cont: list Frame.t -> cont -> Prop :=
+  | sum_cont_nil
+    :
+      sum_cont [] Kstop
+  | sum_cont_cons
+      _fptr _vs k0 _m
+      _targs _tres _cconv
+      (CALL: is_call_cont_strong k0)
+      tl k1
+      (TL: sum_cont tl k1)
+      k2
+      (K: k2 = app_cont k0 k1)
+      cp
+      (FOCUS: is_focus cp)
+      (K0: exists _f _e _C _k, k0 = (Kcall _f _e _C _tres _k) /\ <<WTYK: wtype_cont (prog_comp_env cp) _k>>)
+      (* (WTTGT: exists ge_cp, wt_state ge_cp (Csem.Callstate _fptr (Tfunction _targs _tres _cconv) _vs k0 _m)) *)
+      (WTTGT: wt_state cp (geof cp) (Csem.Callstate _fptr (Tfunction _targs _tres _cconv) _vs k0 _m))
+    :
+      sum_cont ((Frame.mk (CsemC.modsem skenv_link cp)
+                          (Csem.Callstate _fptr (Tfunction _targs _tres _cconv) _vs k0 _m)) :: tl) k2
+  .
+
+  Lemma sum_cont_kstop_inv
+        frs
+        (SUM: sum_cont frs Kstop)
+    :
+      frs = []
+  .
+  Proof.
+    clear - SUM.
+    inv SUM; ss.
+    hexpl app_cont_kstop_inv. clarify.
+  Qed.
+
+  Inductive match_focus_state: Csem.state -> Csem.state -> cont -> Prop :=
+  | reg_state_similar
+      f s k k0 k1 e m
+      (CONT: k = app_cont k1 k0)
+    : match_focus_state (Csem.State f s k e m) (Csem.State f s k1 e m) k0
+  | expr_state_similar
+      f ex k k0 k1 e m
+      (CONT: k = app_cont k1 k0)
+    : match_focus_state (Csem.ExprState f ex k e m) (Csem.ExprState f ex k1 e m) k0
+  | call_sate_similar
+      fptr tyf vargs k k0 k1 m
+      (CONT: k = app_cont k1 k0)
+      (* tyargs tyres cconv *)
+      (* (TYF: classify_fun tyf = fun_case_f tyargs tyres cconv) *)
+      (* (WTVALS: Forall2 val_casted vargs tyargs.(typelist_to_listtype)) *)
+    : match_focus_state (Csem.Callstate fptr tyf vargs k m) (Csem.Callstate fptr tyf vargs k1 m) k0
+  | return_sate_similar
+      vres k k0 k1 m
+      (CONT: k = app_cont k1 k0)
+    : match_focus_state (Csem.Returnstate vres k m) (Csem.Returnstate vres k1 m) k0
+  | stuck_state_similar
+      k0
+    :
+      match_focus_state Csem.Stuckstate Csem.Stuckstate k0
+  .
+  (* Let sum_cont := sum_cont cps sk_link. *)
+  (* variable cp_link cp0 cp1: Csyntax.program. *)
   (* Variable ctx: Syntax.program. *)
   (* Hypothesis FOCUS: link cp0 cp1 = Some cp_link. *)
   (* (* Let prog_src := cp_link.(CsemC.module) :: ctx. *) *)
@@ -89,12 +329,456 @@ Section SIM.
       (* admit "". *)
   Qed.
 
+  (* Lemma size_of_same *)
+  (*       cp t *)
+  (*       (FOC : linkorder_program cp cp_link) *)
+  (*       (EXTENDS : forall id cmp, (prog_comp_env cp) ! id = Some cmp -> (prog_comp_env cp_link) ! id = Some cmp) *)
+  (*       (COMPLETE : complete_type (prog_comp_env cp) t = true) *)
+  (*   : *)
+  (*     sizeof (prog_comp_env cp) t = sizeof (prog_comp_env cp_link) t. *)
+  (* Proof. *)
+  (*   clear -COMPLETE EXTENDS. *)
+  (*   revert t cp cp_link COMPLETE EXTENDS. *)
+  (*   induction t; ss; i; des_ifs; try (by (exploit EXTENDS; eauto; i; Eq; auto)). *)
+  (*   erewrite IHt; eauto. *)
+  (* Qed. *)
+
+  (** Same Lemmas *)
+
+  Lemma field_offset_same
+        cp f0 co delta
+        (FOC : linkorder_program cp cp_link)
+        (EXTENDS : forall id cmp, (prog_comp_env cp) ! id = Some cmp -> (prog_comp_env cp_link) ! id = Some cmp)
+        (COMPLETE : complete_members (prog_comp_env cp) (co_members co) = true)
+    :
+      field_offset (prog_comp_env cp) f0 (co_members co) = Errors.OK delta <->
+      field_offset (prog_comp_env cp_link) f0 (co_members co) = Errors.OK delta.
+  Proof.
+    unfold field_offset in *.
+    remember 0 as n. clear Heqn.
+    revert COMPLETE (* OFFSET *) FOC EXTENDS.
+    revert cp delta f0 n.
+    induction (co_members co) as [| mhd mtl]; try (by ss); i.
+    ss. destruct mhd.
+    assert (ALIGN: (align n (alignof (prog_comp_env cp) t)) = (align n (alignof (prog_comp_env cp_link) t))).
+    { clear -COMPLETE EXTENDS.
+      revert t n cp cp_link COMPLETE EXTENDS.
+      induction t; ss; i; unfold align_attr; des_ifs; auto.
+      - exploit EXTENDS; eauto. i. Eq. auto.
+      - exploit EXTENDS; eauto. i. Eq.
+      - exploit EXTENDS; eauto. i. Eq. auto.
+      - exploit EXTENDS; eauto. i. Eq. }
+    des_ifs.
+    - rewrite ALIGN. auto.
+    - rewrite ALIGN in *.
+      eapply andb_prop in COMPLETE. des; auto.
+      exploit IHmtl; eauto.
+      intros. erewrite H.
+      erewrite <- sizeof_stable; eauto.
+  Qed.
+
+  Lemma sem_add_ptr_int_same1
+        cp f v1 ty1 v2 ty2 ty CC k e m' k1 k2 ty0 si v
+        (WTTGT : wt_state cp
+                   {|
+                     genv_genv := SkEnv.revive (SkEnv.project skenv_link (CSk.of_program signature_of_function cp)) cp;
+                     genv_cenv := prog_comp_env cp |} (ExprState f (CC (Ebinop Oadd (Eval v1 ty1) (Eval v2 ty2) ty)) k e m'))
+        (EXTENDS : forall id cmp, (prog_comp_env cp) ! id = Some cmp -> (prog_comp_env cp_link) ! id = Some cmp)
+        (CTX : context k1 k2 CC)
+        (CLASSADD : classify_add ty1 ty2 = add_case_pi ty0 si)
+    :
+      sem_add_ptr_int (prog_comp_env cp) ty0 si v1 v2 = Some v <->
+      sem_add_ptr_int (prog_comp_env cp_link) ty0 si v1 v2 = Some v.
+  Proof.
+    exploit types_of_context1; eauto. intros [tys [A B]].
+    unfold classify_add in CLASSADD; des_ifs; try (des; clarify); unfold sem_add_ptr_int in *; des_ifs.
+    - erewrite sizeof_wt_stable; eauto; inv WTTGT; ss.
+      unfold typeconv in Heq; des_ifs; ss; clarify.
+      { exploit (WTYE (Tpointer ty0 a1)). eapply B. ss. auto. i. ss. }
+      { exploit (WTYE (Tarray ty0 z a1)). eapply B. ss. auto. i. ss. }
+    - erewrite sizeof_wt_stable; eauto; inv WTTGT; ss.
+      unfold typeconv in Heq; des_ifs; ss; clarify.
+      { exploit (WTYE (Tpointer ty0 a1)). eapply B. ss. auto. i. ss. }
+      { exploit (WTYE (Tarray ty0 z a1)). eapply B. ss. auto. i. ss. }
+  Qed.
+
+  Lemma sem_add_ptr_int_same2
+        cp f v1 ty1 v2 ty2 ty CC k e m' k1 k2 ty0 si v
+        (WTTGT : wt_state cp
+                   {|
+                     genv_genv := SkEnv.revive (SkEnv.project skenv_link (CSk.of_program signature_of_function cp)) cp;
+                     genv_cenv := prog_comp_env cp |} (ExprState f (CC (Ebinop Oadd (Eval v1 ty1) (Eval v2 ty2) ty)) k e m'))
+        (EXTENDS : forall id cmp, (prog_comp_env cp) ! id = Some cmp -> (prog_comp_env cp_link) ! id = Some cmp)
+        (CTX : context k1 k2 CC)
+        (CLASSADD : classify_add ty1 ty2 = add_case_ip si ty0)
+    :
+      sem_add_ptr_int (prog_comp_env cp) ty0 si v2 v1 = Some v <->
+      sem_add_ptr_int (prog_comp_env cp_link) ty0 si v2 v1 = Some v.
+  Proof.
+    exploit types_of_context1; eauto. intros [tys [A B]].
+    unfold classify_add in CLASSADD; des_ifs; try (des; clarify); unfold sem_add_ptr_int in *; des_ifs.
+    - erewrite sizeof_wt_stable; eauto; inv WTTGT; ss.
+      unfold typeconv in Heq0; des_ifs; ss; clarify.
+      { exploit (WTYE (Tpointer ty0 a1)). eapply B. ss. auto. i. ss. }
+      { exploit (WTYE (Tarray ty0 z a1)). eapply B. ss. auto. i. ss. }
+    - erewrite sizeof_wt_stable; eauto; inv WTTGT; ss.
+      unfold typeconv in Heq0; des_ifs; ss; clarify.
+      { exploit (WTYE (Tpointer ty0 a1)). eapply B. ss. auto. i. ss. }
+      { exploit (WTYE (Tarray ty0 z a1)). eapply B. ss. auto. i. ss. }
+  Qed.
+
+  Lemma sem_add_ptr_long_same1
+        cp f v1 ty1 v2 ty2 ty CC k e m' k1 k2 ty0 v
+        (WTTGT : wt_state cp
+                   {|
+                     genv_genv := SkEnv.revive (SkEnv.project skenv_link (CSk.of_program signature_of_function cp)) cp;
+                     genv_cenv := prog_comp_env cp |} (ExprState f (CC (Ebinop Oadd (Eval v1 ty1) (Eval v2 ty2) ty)) k e m'))
+        (EXTENDS : forall id cmp, (prog_comp_env cp) ! id = Some cmp -> (prog_comp_env cp_link) ! id = Some cmp)
+        (CTX : context k1 k2 CC)
+        (CLASSADD : classify_add ty1 ty2 = add_case_pl ty0)
+    :
+      sem_add_ptr_long (prog_comp_env cp) ty0 v1 v2 = Some v <->
+      sem_add_ptr_long (prog_comp_env cp_link) ty0 v1 v2 = Some v.
+  Proof.
+    exploit types_of_context1; eauto. intros [tys [A B]].
+    unfold classify_add in CLASSADD; des_ifs; try (des; clarify); unfold sem_add_ptr_long in *; des_ifs.
+    - erewrite sizeof_wt_stable; eauto; inv WTTGT; ss.
+      unfold typeconv in Heq; des_ifs; ss; clarify.
+      { exploit (WTYE (Tpointer ty0 a1)). eapply B. ss. auto. i. ss. }
+      { exploit (WTYE (Tarray ty0 z a1)). eapply B. ss. auto. i. ss. }
+    - erewrite sizeof_wt_stable; eauto; inv WTTGT; ss.
+      unfold typeconv in Heq; des_ifs; ss; clarify.
+      { exploit (WTYE (Tpointer ty0 a1)). eapply B. ss. auto. i. ss. }
+      { exploit (WTYE (Tarray ty0 z a1)). eapply B. ss. auto. i. ss. }
+  Qed.
+
+  Lemma sem_add_ptr_long_same2
+        cp f v1 ty1 v2 ty2 ty CC k e m' k1 k2 ty0 v
+        (WTTGT : wt_state cp
+                   {|
+                     genv_genv := SkEnv.revive (SkEnv.project skenv_link (CSk.of_program signature_of_function cp)) cp;
+                     genv_cenv := prog_comp_env cp |} (ExprState f (CC (Ebinop Oadd (Eval v1 ty1) (Eval v2 ty2) ty)) k e m'))
+        (EXTENDS : forall id cmp, (prog_comp_env cp) ! id = Some cmp -> (prog_comp_env cp_link) ! id = Some cmp)
+        (CTX : context k1 k2 CC)
+        (CLASSADD : classify_add ty1 ty2 = add_case_lp ty0)
+    :
+      sem_add_ptr_long (prog_comp_env cp) ty0 v2 v1 = Some v <->
+      sem_add_ptr_long (prog_comp_env cp_link) ty0 v2 v1 = Some v.
+  Proof.
+    exploit types_of_context1; eauto. intros [tys [A B]].
+    unfold classify_add in CLASSADD; des_ifs; try (des; clarify); unfold sem_add_ptr_long in *; des_ifs.
+    - des_ifs; erewrite sizeof_wt_stable; eauto; inv WTTGT; ss.
+      unfold typeconv in Heq0; des_ifs; ss; clarify.
+      { exploit (WTYE (Tpointer ty0 a1)). eapply B. ss. auto. i. ss. }
+      { exploit (WTYE (Tarray ty0 z a1)). eapply B. ss. auto. i. ss. }
+    - des_ifs; erewrite sizeof_wt_stable; eauto; inv WTTGT; ss.
+      unfold typeconv in Heq0; des_ifs; ss; clarify.
+      { exploit (WTYE (Tpointer ty0 a1)). eapply B. ss. auto. i. ss. }
+      { exploit (WTYE (Tarray ty0 z a1)). eapply B. ss. auto. i. ss. }
+  Qed.
+
+  Lemma sem_sub_same
+        cp f v1 ty1 v2 ty2 ty CC k e m' k1 k2 k0 v
+        (WTSRC : wt_state cp_link
+                   {|
+                     genv_genv := SkEnv.revive (SkEnv.project skenv_link (CSk.of_program signature_of_function cp_link)) cp_link;
+                     genv_cenv := prog_comp_env cp_link |}
+                   (ExprState f (CC (Ebinop Osub (Eval v1 ty1) (Eval v2 ty2) ty)) (app_cont k k0) e m'))
+        (WTTGT : wt_state cp
+                   {|
+                     genv_genv := SkEnv.revive (SkEnv.project skenv_link (CSk.of_program signature_of_function cp)) cp;
+                     genv_cenv := prog_comp_env cp |} (ExprState f (CC (Ebinop Osub (Eval v1 ty1) (Eval v2 ty2) ty)) k e m'))
+        (EXTENDS : forall id cmp, (prog_comp_env cp) ! id = Some cmp -> (prog_comp_env cp_link) ! id = Some cmp)
+        (CTX : context k1 k2 CC)
+    :
+      sem_sub (prog_comp_env cp) v1 ty1 v2 ty2 m' = Some v <->
+      sem_sub (prog_comp_env cp_link) v1 ty1 v2 ty2 m' = Some v.
+  Proof.
+    exploit types_of_context1; eauto. intros [tys [A B]].
+    unfold sem_sub.
+    (* des_ifs; erewrite sizeof_wt_stable in *; eauto; inv WTTGT; inv WTSRC; ss; *)
+    (*   unfold classify_sub in Heq; destruct ty1; destruct ty2; des_ifs; ss; clarify; des_ifs; *)
+    (*     try (by (exploit (WTYE (Tpointer ty0 a)); try eapply B; ss; auto; i; ss)); *)
+    (*     try (by (exploit (WTYE (Tarray ty0 z a)); try eapply B; ss; auto; i; ss)); *)
+    (*     try (by (exploit (WTYE0 (Tpointer ty0 a)); try eapply B; ss; auto; i; ss)); *)
+    (*     try (by (exploit (WTYE0 (Tarray ty0 z a)); try eapply B; ss; auto; i; ss)). *)
+    admit "".
+  Qed.
+
+  Lemma sem_add_same
+        cp f v1 ty1 v2 ty2 ty CC k e m' k1 k2 v
+        (WTTGT : wt_state cp
+                   {|
+                     genv_genv := SkEnv.revive (SkEnv.project skenv_link (CSk.of_program signature_of_function cp)) cp;
+                     genv_cenv := prog_comp_env cp |} (ExprState f (CC (Ebinop Oadd (Eval v1 ty1) (Eval v2 ty2) ty)) k e m'))
+        (EXTENDS : forall id cmp, (prog_comp_env cp) ! id = Some cmp -> (prog_comp_env cp_link) ! id = Some cmp)
+        (CTX : context k1 k2 CC)
+    :
+      sem_add (prog_comp_env cp) v1 ty1 v2 ty2 m' = Some v <->
+      sem_add (prog_comp_env cp_link) v1 ty1 v2 ty2 m' = Some v.
+  Proof.
+    unfold sem_add in *. des_ifs.
+    - exploit sem_add_ptr_int_same1; eauto.
+    - exploit sem_add_ptr_long_same1; eauto.
+    - exploit sem_add_ptr_int_same2; eauto.
+    - exploit sem_add_ptr_long_same2; eauto.
+  Qed.
+
+  Lemma free_list_exists
+        cp m e m' (* k1 k2 *) (* CC *)
+        (WTENV: forall id blk ty, e ! id = Some (blk, ty) -> wt_type (prog_comp_env cp) ty)
+        (* (WTTGT : wt_state *)
+        (*            {| *)
+        (*              genv_genv := SkEnv.revive *)
+        (*                             (SkEnv.project skenv_link (CSk.of_program signature_of_function cp)) cp; *)
+        (*              genv_cenv := prog_comp_env cp |} (Csem.State f Sskip k e m)) *)
+        (EXTENDS : forall (id : positive) (cmp : composite),
+            (prog_comp_env cp) ! id = Some cmp -> (prog_comp_env cp_link) ! id = Some cmp)
+        (FREE : Mem.free_list m (blocks_of_env (geof cp_link) e) = Some m')
+    :
+      Mem.free_list m (blocks_of_env (geof cp) e) = Some m'.
+      (* exists m'', Mem.free_list m (blocks_of_env (geof cp) e) = Some m''. *)
+  Proof.
+    unfold blocks_of_env, block_of_binding in *. ss.
+    assert (WTENV0: forall p blk ty, In (p, (blk, ty)) (PTree.elements e) -> wt_type (prog_comp_env cp) ty).
+    { i. exploit PTree.elements_complete; eauto. }
+    revert (* CTX *) FREE EXTENDS WTENV WTENV0. revert (* CC k1 k2 *) m' cp m.
+    induction (PTree.elements e); ss. ii; eauto.
+    i. des_ifs.
+    - erewrite sizeof_wt_stable in Heq0; eauto. Eq.
+      exploit IHl; eauto.
+      { specialize (WTENV0 p b t). exploit WTENV0; eauto. }
+    - erewrite sizeof_wt_stable in Heq0; eauto. Eq.
+      { specialize (WTENV0 p b t). exploit WTENV0; eauto. }
+  Qed.
+
+  Lemma free_list_same
+        cp m e m' (* k1 k2 *) (* CC *)
+        (WTENV: forall id blk ty, e ! id = Some (blk, ty) -> wt_type (prog_comp_env cp) ty)
+        (* (WTTGT : wt_state *)
+        (*            {| *)
+        (*              genv_genv := SkEnv.revive *)
+        (*                             (SkEnv.project skenv_link (CSk.of_program signature_of_function cp)) cp; *)
+        (*              genv_cenv := prog_comp_env cp |} (Csem.State f Sskip k e m)) *)
+        (EXTENDS : forall (id : positive) (cmp : composite),
+            (prog_comp_env cp) ! id = Some cmp -> (prog_comp_env cp_link) ! id = Some cmp)
+        (FREE : Mem.free_list m
+                              (blocks_of_env
+                                 {|
+                                   genv_genv := SkEnv.revive
+                                                  (SkEnv.project skenv_link (CSk.of_program signature_of_function cp)) cp;
+                                   genv_cenv := prog_comp_env cp |} e) = Some m')
+        (* (CTX : context k1 k2 CC) *)
+    :
+      Mem.free_list m
+                    (blocks_of_env
+                       {|
+                         genv_genv := SkEnv.revive
+                                        (SkEnv.project skenv_link (CSk.of_program signature_of_function cp_link))
+                                        cp_link;
+                         genv_cenv := prog_comp_env cp_link |} e) = Some m'.
+  Proof.
+    unfold blocks_of_env, block_of_binding in *. ss.
+    assert (WTENV0: forall p blk ty, In (p, (blk, ty)) (PTree.elements e) -> wt_type (prog_comp_env cp) ty).
+    { i. exploit PTree.elements_complete; eauto. }
+    revert (* CTX *) FREE EXTENDS WTENV WTENV0. revert (* CC k1 k2 *) m' cp m.
+    induction (PTree.elements e); ss. ii.
+    des_ifs.
+    - erewrite <- sizeof_wt_stable in Heq0; eauto. Eq.
+      exploit IHl; eauto.
+      { specialize (WTENV0 p b t). exploit WTENV0; eauto. }
+    - erewrite <- sizeof_wt_stable in Heq0; eauto. Eq.
+      { specialize (WTENV0 p b t). exploit WTENV0; eauto. }
+  Qed.
+
+  Lemma alignof_blockcopy_wt_stable:
+    forall t ce ce' (extends: forall id co, ce!id = Some co -> ce'!id = Some co),
+    wt_type ce t = true ->
+    alignof_blockcopy ce t = alignof_blockcopy ce' t.
+  Proof.
+    induction t; simpl; intros; auto.
+    - destruct (ce!i) as [co|] eqn:E; try discriminate.
+      erewrite extends by eauto. auto.
+    - destruct (ce!i) as [co|] eqn:E; try discriminate.
+      erewrite extends by eauto. auto.
+  Qed.
+
+  Lemma alloc_variables_same
+        cp f m e m1
+        (WT : Forall (fun t : type => wt_type (prog_comp_env cp) t) (map snd (fn_params f ++ fn_vars f)))
+        (EXTENDS: forall id cmp, (prog_comp_env cp) ! id = Some cmp -> (prog_comp_env cp_link) ! id = Some cmp)
+        (ALLOC : alloc_variables (geof cp) empty_env m (fn_params f ++ fn_vars f) e m1)
+    :
+      alloc_variables (geof cp_link) empty_env m (fn_params f ++ fn_vars f) e m1.
+  Proof.
+    assert (EMPTY:forall i blk ty, empty_env ! i = Some (blk, ty) -> wt_type (prog_comp_env cp) ty).
+    { ii. erewrite PTree.gempty in H. clarify. }
+    remember (fn_params f ++ fn_vars f) as l.
+    remember empty_env as ev.
+    clear Heqev.
+    clear Heql.
+    ginduction l; i; ss; inv ALLOC.
+    - econs.
+    - econs; eauto.
+      + ss. erewrite <- sizeof_wt_stable; eauto.
+        inv WT. eauto.
+      + eapply IHl; eauto.
+        { inv WT; eauto. }
+        i. destruct (classic (id = i)).
+        { subst. rewrite PTree.gss in H. clarify. inv WT; auto. }
+        rewrite PTree.gso in H; eauto.
+  Qed.
+
+  Lemma bind_parameters_same
+        cp f vargs  m1 e m2
+        (WT : Forall (fun t : type => wt_type (prog_comp_env cp) t) (map snd (fn_params f ++ fn_vars f)))
+        (EXTENDS: forall id cmp, (prog_comp_env cp) ! id = Some cmp -> (prog_comp_env cp_link) ! id = Some cmp)
+        (BIND : bind_parameters skenv_link (geof cp) e m1 (fn_params f) vargs m2)
+    :
+      bind_parameters skenv_link (geof cp_link) e m1 (fn_params f) vargs m2.
+  Proof.
+    assert (EMPTY:forall i blk ty, empty_env ! i = Some (blk, ty) -> wt_type (prog_comp_env cp) ty).
+    { ii. erewrite PTree.gempty in H. clarify. }
+    remember (fn_params f) as l.
+    clear Heql.
+    ginduction l; i; ss; inv BIND.
+    - econs.
+    - econs; eauto.
+      + inv H3; try (by econs; eauto).
+        inv WT.
+        econs 3; ss; eauto;
+          try (by (erewrite <- alignof_blockcopy_wt_stable; eauto));
+          try (by (erewrite <- sizeof_wt_stable; eauto)).
+      + exploit IHl; eauto.
+        { instantiate (1:=f). ss. inv WT. eauto. }
+  Qed.
+  
+  Lemma preservation_alloc
+        cp_top m1 e l m0
+        (FOCUS1 : is_focus cp_top)
+        (ALLOC : alloc_variables ge_cp_link empty_env m0
+                   l e m1)
+        (COMP : Forall (fun t : type => wt_type (prog_comp_env cp_top) t)
+                       (map snd l))
+    :
+      alloc_variables (geof cp_top) empty_env m0 l e m1.
+  Proof.
+    induction ALLOC.
+    - econs.
+    - ss. inv COMP.
+      assert (forall id co, (prog_comp_env cp_top) ! id = Some co -> (prog_comp_env cp_link) ! id = Some co).
+      { i. exploit link_list_linkorder; eauto. intro ORD. r in ORD. rewrite Forall_forall in ORD.
+        exploit ORD; et. intro ORD0. ss. rr in ORD0. des. et.
+      }
+      exploit sizeof_wt_stable; eauto.
+      i. eapply IHALLOC in H3.
+      econs; eauto. ss. rewrite H1. eauto.
+  Qed.
+
+  Lemma preservation_bind_param
+        cp_top m1 e l l' m2 vs_arg
+        (FOCUS1 : is_focus cp_top)
+        (PARAM : bind_parameters skenv_link ge_cp_link e m1 l vs_arg m2)
+        (COMP : Forall (fun t : type => wt_type (prog_comp_env cp_top) t) (map snd (l ++ l')))
+    :
+      bind_parameters skenv_link (geof cp_top) e m1 l vs_arg m2.
+  Proof.
+    induction PARAM.
+    - econs.
+    - ss. inv COMP.
+      exploit IHPARAM; eauto. i. econs; eauto.
+      inv H0.
+      * econs; eauto.
+      * econs 2; eauto.
+      * assert (forall id co, (prog_comp_env cp_top) ! id = Some co -> (prog_comp_env cp_link) ! id = Some co).
+        { i. exploit link_list_linkorder; eauto. intro ORD. r in ORD. rewrite Forall_forall in ORD.
+          exploit ORD; et. intro ORD0. ss. rr in ORD0. des_safe. et.
+        }
+        des; econs 3; eauto; ss;
+          destruct ty; ss; des_ifs; exploit H0; eauto; i; rewrite Heq0 in H10; inv H10; eauto.
+  Qed.
+
+  (* Scheme find_label_mut := Minimality for find_label Sort Prop *)
+  (*   with find_label_ls_mut := Minimality for find_label_ls Sort Prop. *)
+
+  Scheme statement_mut := Induction for statement Sort Prop
+    with labeled_statements_mut := Induction for labeled_statements Sort Prop.
+
+  Lemma find_label_same_None
+        tl_tgt k0 lbl s k
+        (SUM : sum_cont tl_tgt k0)
+        (LABEL : find_label lbl s k = None)
+    :
+      find_label lbl s (app_cont k k0) = None.
+  Proof.
+    revert_until s. revert s lbl k0 tl_tgt.
+    eapply (statement_mut (fun s => forall lbl k0 tl_tgt k,
+                               sum_cont tl_tgt k0 ->
+                               find_label lbl s k = None -> find_label lbl s (app_cont k k0) = None)
+                          (fun sl => forall K lbl k0 tl_tgt k,
+                               sum_cont tl_tgt k0 ->
+                               find_label_ls lbl sl k = None -> find_label_ls lbl sl (app_cont k k0) = None)
+           ); ss; i; ss; des_ifs; (try exploit H; eauto; ss; i; try Eq).
+    - exploit H1; eauto. i. ss. Eq.
+    - exploit H0; eauto.
+  Qed.
+
+  Lemma find_label_same
+        tl_tgt k0 lbl s k s' k'
+        (SUM : sum_cont tl_tgt k0)
+        (LABEL : find_label lbl s k = Some (s', k'))
+    :
+      find_label lbl s (app_cont k k0) = Some (s', app_cont k' k0).
+  Proof.
+    revert SUM. revert_until s.
+    revert lbl k0 tl_tgt. clear INCL_FOCUS.
+    eapply (statement_mut (fun s =>  forall lbl k0 tl_tgt k s' k',
+                               find_label lbl s k = Some (s', k') ->
+                               sum_cont tl_tgt k0 -> find_label lbl s (app_cont k k0) = Some (s', app_cont k' k0))
+                          (fun sl => forall lbl k0 tl_tgt k s' k',
+                               sum_cont tl_tgt k0 ->
+                               find_label_ls lbl sl k = Some (s', k') -> find_label_ls lbl sl (app_cont k k0) = Some (s', app_cont k' k0))
+           ); ss.
+    - i. des_ifs.
+      + exploit H; eauto; ss; i; Eq; auto.
+      + exploit find_label_same_None; eauto; ss. i. Eq.
+      + exploit H; eauto; ss; i; Eq; auto.
+      + exploit H0; eauto; ss; i; Eq; auto.
+    - i. des_ifs.
+      + exploit H; eauto; ss; i; Eq; auto.
+      + exploit find_label_same_None; eauto; ss. i. Eq.
+      + exploit H; eauto; ss; i; Eq; auto.
+      + exploit H0; eauto; ss; i; Eq; auto.
+    - i. exploit H; eauto.
+    - i. exploit H; eauto.
+    - i. des_ifs.
+      + i. exploit H; eauto. ss. i. Eq. auto.
+      + exploit find_label_same_None; eauto; ss. i. Eq.
+      + exploit find_label_same_None; try eapply Heq0; eauto; ss. i. Eq.
+      + i. exploit H; eauto. ss. i. Eq.
+      + i. exploit H1; eauto. ss. i. Eq. auto.
+      + exploit find_label_same_None; try eapply Heq2; eauto; ss. i. Eq.
+      + i. exploit H; eauto. ss. i. Eq.
+      + i. exploit H1; eauto. ss. i. Eq.
+      + i. exploit H0; eauto.
+    - i. exploit H; eauto.
+    - i. des_ifs. exploit H; eauto.
+    - i. des_ifs.
+      + exploit H; eauto; ss; i; Eq; auto.
+      + exploit find_label_same_None; eauto; ss. i. Eq.
+      + exploit H; eauto; ss; i; Eq; auto.
+      + exploit H0; eauto; ss; i; Eq; auto.
+  Qed.
+
+  Hypothesis WFSRC: forall md : Mod.t, In md prog_src -> Sk.wf md.
+  Hypothesis WFTGT: forall md : Mod.t, In md prog_tgt -> Sk.wf md.
+
   Lemma match_focus_state_bsim
         cst_src0 cst_tgt0 cst_tgt1 k0 cp tr
         (ST: match_focus_state cst_src0 cst_tgt0 k0)
-        (FOC: linkorder cp cp_link)
-        (WTSRC: wt_state (geof cp_link) cst_src0)
-        (WTTGT: wt_state (geof cp) cst_tgt0)
+        (ISFOC: is_focus cp)
+        (WTSRC: wt_state cp_link (geof cp_link) cst_src0)
+        (WTTGT: wt_state cp (geof cp) cst_tgt0)
         (STEP: Csem.step skenv_link (geof cp) cst_tgt0 tr cst_tgt1)
         tl_tgt
         (SUM: sum_cont tl_tgt k0)
@@ -103,71 +787,488 @@ Section SIM.
       <<STEP: Csem.step skenv_link (geof cp_link) cst_src0 tr (matched_state_source cst_tgt1 k0)>>
   .
   Proof.
+    assert (FOC: linkorder cp cp_link).
+    { exploit link_list_linkorder; eauto. i. rr in H.
+      rewrite Forall_forall in H. exploit H; eauto. }
     pose cst_tgt1 as XXX.
     assert(EXTENDS: forall id cmp (IN: (prog_comp_env cp) ! id = Some cmp),
               <<IN: (prog_comp_env cp_link) ! id = Some cmp>>).
-    { admit "ez". }
+    {
+      Local Transparent Linker_program. ss.
+      unfold link_program in *. des_ifs.
+      Local Transparent Linker_prog. ss.
+      unfold linkorder_program in FOC. inv FOC. eauto. }
     unfold NW in *. (* TODO: Hint Unfold NW does not work !!! *)
     rr in STEP. des.
-    - left.
-      inv STEP; inv ST; econs; eauto.
+    - inv STEP; inv ST. (* left; econs; eauto. *)
       + (* lred *)
-        inv H; econs; ss; eauto.
-        * admit "ez - genv".
-        * hexploit (prog_comp_env_eq cp); et. intro X.
+        left; econs; eauto.
+        inv H; try (by econs; ss; eauto).
+        * econs 2; eauto. ss.
+          unfold Genv.find_symbol in *. ss. rewrite MapsC.PTree_filter_key_spec in *.
+          des_ifs. inv FOC. inv H. ss. des.
+          rewrite CSk.of_program_defs in *.
+          assert (defs cp x) by auto. rewrite <- defs_prog_defmap in *. des.
+          exploit H6; eauto. i. des.
+          assert (defs cp_link x).
+          { rewrite <- defs_prog_defmap. exists gd2. eauto. } clarify.
+        * econs; ss; eauto.
+          hexploit (prog_comp_env_eq cp); et. intro X.
           exploit build_composite_env_consistent; et. intro Y.
           exploit co_consistent_complete; et. intro Z.
-          admit "field_offset: make lemma".
+          erewrite <- field_offset_same; eauto.
       + (* rred *)
+        left. econs; eauto.
         rename C into CC.
+        inversion WTTGT; subst; ss. exploit types_of_context1; eauto. intros [tys [A B]].
         inv H; try (econs; ss; eauto); ss.
         * destruct op; ss.
-          { admit "sem_binary_operation: make lemma". }
-          { admit "sem_binary_operation: make lemma". }
+          { erewrite <- sem_add_same; eauto. }
+          { erewrite <- sem_sub_same; eauto. }
         * rpapply red_sizeof; eauto. ss.
-          erewrite <- sizeof_stable; eauto.
-          clear - H0 WTTGT.
-          admit "strengthen typechecker".
+          erewrite sizeof_wt_stable; eauto.
+          clear - H0 WTTGT WTYE B.
+          exploit (WTYE ty1); eauto.
+          eapply B. ss. auto.
         * rpapply red_alignof; eauto. ss.
-          admit "strengthen typechecker".
+          erewrite alignof_wt_stable; eauto.
+          clear - H0 WTTGT WTYE B.
+          exploit (WTYE ty1); eauto.
+          eapply B. ss. auto.
         * inv H2; try (by econs; eauto).
           econs 3; ss; eauto.
-          admit "strengthen typechecker and make lemma".
-          admit "strengthen typechecker".
-          admit "strengthen typechecker".
-          admit "strengthen typechecker".
-      + ii. eapply H0.
+          { erewrite <- alignof_blockcopy_wt_stable; eauto.
+            exploit (WTYE); try eapply B; ss; auto; i; ss. }
+          { erewrite <- alignof_blockcopy_wt_stable; eauto.
+            exploit (WTYE); try eapply B; ss; auto; i; ss. }
+          { erewrite <- sizeof_wt_stable; eauto.
+            inv WTTGT; ss. exploit (WTYE ty1); eauto. eapply B. ss. auto. }
+          { erewrite <- sizeof_wt_stable; eauto.
+            inv WTTGT; ss. exploit (WTYE ty1); eauto. eapply B. ss. auto. }
+      + left. econs; eauto.
+      + left. econs; eauto. ii. eapply H0.
         inv H1.
         * econs 1; eauto.
         * econs 2; eauto.
-        * econs 3; eauto.
-          admit "lred progress (make a lemma)".
-        * econs 4; eauto.
-          admit "rred progress (make a lemma)".
+        * inv H2.
+          { econs 3; eauto.
+            instantiate (1:= m'). instantiate (1:=(Eloc b Ptrofs.zero ty)). econs; eauto. }
+          { ss. econs 3; eauto. econs 2; eauto. ss.
+            inv WTTGT; ss.
+            exploit context_compose. eapply H. eauto. i.
+            exploit wt_rvalue_wt_expr; eauto. ss. eauto. i.
+            inv H5. ss. rewrite WTTENV in *. inv H7. Eq. eauto. }
+          { econs 3; eauto. ss. econs 3; eauto. }
+          { exploit context_compose. eapply H. eauto. i.
+            exploit types_of_context1; eauto. intros [tys [A B]].
+            inv WTTGT. ss. exploit (WTYE (Tstruct id a)).
+            eapply B. ss. auto. i. inv H5. des_ifs.
+            econs 3; eauto. ss. econs 4; eauto; ss.
+            erewrite field_offset_same; eauto. exploit EXTENDS; eauto. i. Eq. eauto.
+            hexploit (prog_comp_env_eq cp); et. intro X.
+            exploit build_composite_env_consistent; et. intro Y.
+            exploit co_consistent_complete; et. }
+          { exploit context_compose. eapply H. eauto. i.
+            exploit types_of_context1; eauto. intros [tys [A B]].
+            inv WTTGT. ss. exploit (WTYE (Tunion id a)).
+            eapply B. ss. auto. i. inv H4. des_ifs.
+            econs 3; eauto. ss. econs 5; eauto. }
+          (* admit "lred progress (make a lemma)". *)
+        * inv H2; try (by (econs 4; eauto; econs; eauto)).
+          { econs 4; eauto. econs 4; eauto. ss. unfold sem_binary_operation in *. des_ifs; eauto.
+            - exploit context_compose. eapply H. eapply H3. i.
+              erewrite sem_add_same; eauto. ss. eauto.
+            - exploit context_compose. eapply H. eapply H3. i.
+              erewrite sem_sub_same; try eapply H2. eauto. eapply WTSRC. eapply WTTGT. eauto. }
+          { exploit context_compose. eapply H. eauto. i.
+            inversion WTTGT; subst; ss. exploit types_of_context1; eauto. intros [tys [A B]].
+            inv H4; econs 4; eauto; econs; eauto.
+            - econs 1; eauto.
+            - econs 2; eauto.
+            - econs 3; eauto; ss.
+              + erewrite alignof_blockcopy_wt_stable; eauto.
+                exploit (WTYE); try eapply B; ss; auto; i; ss.
+              + erewrite alignof_blockcopy_wt_stable; eauto.
+                exploit (WTYE); try eapply B; ss; auto; i; ss.
+              + erewrite sizeof_wt_stable; eauto.
+                exploit (WTYE ty1); eauto. eapply B. ss. auto.
+              + erewrite sizeof_wt_stable; eauto.
+                exploit (WTYE ty1); eauto. eapply B. ss. auto. }
         * econs 5; eauto.
     - right.
       inv STEP; inv ST; try (by econs; eauto).
       + ss. rpapply step_return_0; eauto.
-        * admit "strengthen typechecker".
+        * inv WTTGT; ss.
+          exploit free_list_same; eauto.
         * erewrite call_cont_app_cont; et.
       + ss. rpapply step_return_2; eauto.
-        * admit "strengthen typechecker".
+        * inv WTTGT; ss.
+          exploit free_list_same; eauto.
         * erewrite call_cont_app_cont; et.
       + ss. eapply step_skip_call; eauto.
         * exploit Cstrategy.is_call_cont_call_cont; et. intro T.
           (* TODO: make lemma *)
           clear - H T SUM. unfold is_call_cont in H. des_ifs. ss. inv SUM; ss. des; clarify.
-        * admit "strengthen typechecker".
+        * inv WTTGT; ss.
+          exploit free_list_same; eauto.
       + ss. eapply step_goto; et.
-        clear - SUM H.
+        clear -H SUM.
         erewrite <- call_cont_app_cont; et.
-        admit "make lemma".
-      + ss. eapply step_internal_function; et.
-        * admit "quantify NCALLTGT".
-        * admit "strengthen typechecker".
-        * admit "strengthen typechecker".
-      + exfalso.
-        admit "quantify NCALLSRC".
-  Admitted.
+        remember (fn_body f) as s. clear Heqs.
+        remember (call_cont k) as k1. clear Heqk1.
+        exploit find_label_same; eauto.
+      + inversion WTTGT; subst; ss.
+        exploit WTLOCAL; eauto. intros WT.
+        eapply step_internal_function; et.
+        * ss. unfold Genv.find_funct in *. des_ifs. rewrite Genv.find_funct_ptr_iff in *.
+          admit "ez".
+        * exploit alloc_variables_same; eauto.
+        * exploit bind_parameters_same; eauto.
+      + destruct (classic (is_external_ef ef)) eqn:EXT.
+        * unfold Genv.find_funct in *. des_ifs. rewrite Genv.find_funct_ptr_iff in *.
+          exploit CSkEnv.project_revive_no_external; eauto.
+          eapply SkEnv.load_skenv_wf; eauto.
+          { eapply link_list_preserves_wf_sk; eauto. }
+          clarify.
+        * eapply step_external_function; eauto.
+          { instantiate (1:=cc). instantiate (1 := tres). instantiate (1 := targs).
+            admit "ez". }
+          { ss. }
+        Unshelve. all: auto.
+  Qed.
+
+  Lemma match_focus_state_progress
+        cst_src0 cst_tgt0 cst_src1 k0 cp tr
+        (NCALLTGT : ~ exists args, at_external skenv_link cp cst_tgt0 args)
+        (NCALLSRC : ~ exists args, at_external skenv_link cp_link cst_src0 args)
+        (NRETTGT : ~ ModSem.is_return (modsem skenv_link cp) cst_tgt0)
+        (NRETSRC : ~ ModSem.is_return (modsem skenv_link cp_link) cst_src0)
+        (ST: match_focus_state cst_src0 cst_tgt0 k0)
+        (ISFOC: is_focus cp)
+        (WTSRC: wt_state cp_link (geof cp_link) cst_src0)
+        (WTTGT: wt_state cp (geof cp) cst_tgt0)
+        (STEP: Csem.step skenv_link (geof cp_link) cst_src0 tr cst_src1)
+        tl_tgt
+        (SUM: sum_cont tl_tgt k0)
+    :
+      (<<STEP: exists cst_tgt1, Csem.step skenv_link (geof cp) cst_tgt0 tr cst_tgt1>>).
+  Proof.
+    assert (FOC: linkorder cp cp_link).
+    { exploit link_list_linkorder; eauto. i. rr in H.
+      rewrite Forall_forall in H. exploit H; eauto. }
+    pose cst_src1 as XXX.
+    assert(EXTENDS: forall id cmp (IN: (prog_comp_env cp) ! id = Some cmp),
+              <<IN: (prog_comp_env cp_link) ! id = Some cmp>>).
+    {
+      Local Transparent Linker_program. ss.
+      unfold link_program in *. des_ifs.
+      Local Transparent Linker_prog. ss.
+      unfold linkorder_program in FOC. inv FOC. eauto. }
+    unfold NW in *. (* TODO: Hint Unfold NW does not work !!! *)
+    rr in STEP. des.
+    - inv STEP; inv ST. (* left; econs; eauto. *)
+      + (* lred *)
+        inv H.
+        * eexists. do 2 econs; eauto. econs; eauto.
+        * eexists. do 2 econs; eauto. econs 2; eauto.
+          ss. inv WTTGT; ss.
+          exploit wt_rvalue_wt_expr; eauto. ss. eauto. i.
+          inv H. ss. rewrite WTTENV in *. inv H4. Eq. eauto.
+        * eexists. do 2 econs; eauto. econs 3; eauto.
+        * inversion WTTGT; subst; ss. exploit types_of_context1; eauto. intros [tys [A B]].
+          inv WTTGT; ss. exploit (WTYE (Tstruct id a0)).
+          eapply B. ss. auto. i. inv H. des_ifs.
+          eexists. do 2 econs; eauto. econs 4; eauto; ss.
+          erewrite field_offset_same; eauto. exploit EXTENDS; eauto. i. Eq. eauto.
+          hexploit (prog_comp_env_eq cp); et. intro X.
+          exploit build_composite_env_consistent; et. intro Y.
+          exploit co_consistent_complete; et.
+        * exploit types_of_context1; eauto. intros [tys [A B]].
+          inv WTTGT. ss. exploit (WTYE (Tunion id a0)).
+          eapply B. ss. auto. i. inv H. des_ifs.
+          eexists. do 2 econs; eauto. econs 5; eauto.
+      + (* rred *)
+        rename C into CC.
+        inversion WTTGT; subst; ss. exploit types_of_context1; eauto. intros [tys [A B]].
+        inv H; try by (eexists; econs; econs 2; eauto; econs; eauto).
+        * eexists; econs; econs 2; eauto; econs; eauto.
+          destruct op; ss; eauto.
+          { erewrite sem_add_same; eauto. }
+          { erewrite sem_sub_same; eauto. }
+        * eexists. econs. econs 2; eauto. econs; eauto.
+          inv H2; try (by econs; eauto).
+          econs 3; ss; eauto.
+          { erewrite alignof_blockcopy_wt_stable; eauto.
+            exploit (WTYE); try eapply B; ss; auto; i; ss. }
+          { erewrite alignof_blockcopy_wt_stable; eauto.
+            exploit (WTYE); try eapply B; ss; auto; i; ss. }
+          { erewrite sizeof_wt_stable; eauto.
+            inv WTTGT; ss. exploit (WTYE ty1); eauto. eapply B. ss. auto. }
+          { erewrite sizeof_wt_stable; eauto.
+            inv WTTGT; ss. exploit (WTYE ty1); eauto. eapply B. ss. auto. }
+      + eexists. econs. econs 3; eauto.
+      + eexists. econs. econs 4; eauto. ii. eapply H0.
+        inv H1.
+        * econs 1; eauto.
+        * econs 2; eauto.
+        * inv H2.
+          { econs 3; eauto.
+            instantiate (1:= m'). instantiate (1:=(Eloc b Ptrofs.zero ty)). econs; eauto. }
+          { ss. econs 3; eauto. econs 2; eauto. ss.
+            admit "ez". }
+          { econs 3; eauto. ss. econs 3; eauto. }
+          { exploit context_compose. eapply H. eauto. i.
+            exploit types_of_context1; eauto. intros [tys [A B]].
+            inv WTTGT. ss. exploit (WTYE (Tstruct id a)).
+            eapply B. ss. auto. i. inv H5. des_ifs.
+            econs 3; eauto. ss. econs 4; eauto; ss.
+            erewrite <- field_offset_same; eauto. exploit EXTENDS; eauto. i. Eq. eauto.
+            hexploit (prog_comp_env_eq cp); et. intro X.
+            exploit build_composite_env_consistent; et. intro Y.
+            exploit co_consistent_complete; et. }
+          { exploit context_compose. eapply H. eauto. i.
+            exploit types_of_context1; eauto. intros [tys [A B]].
+            inv WTTGT. ss. exploit (WTYE (Tunion id a)).
+            eapply B. ss. auto. i. inv H4. des_ifs.
+            econs 3; eauto. ss. econs 5; eauto. }
+          (* admit "lred progress (make a lemma)". *)
+        * inv H2; try (by (econs 4; eauto; econs; eauto)).
+          { econs 4; eauto. econs 4; eauto. ss. unfold sem_binary_operation in *. des_ifs; eauto.
+            - exploit context_compose. eapply H. eapply H3. i.
+              erewrite <- sem_add_same; eauto. ss. eauto.
+            - exploit context_compose. eapply H. eapply H3. i.
+              erewrite <- sem_sub_same; try eapply H2. eauto. eapply WTSRC. eapply WTTGT. eauto. }
+          { exploit context_compose. eapply H. eauto. i.
+            inversion WTTGT; subst; ss. exploit types_of_context1; eauto. intros [tys [A B]].
+            inv H4; econs 4; eauto; econs; eauto.
+            - econs 1; eauto.
+            - econs 2; eauto.
+            - econs 3; eauto; ss.
+              + erewrite <- alignof_blockcopy_wt_stable; eauto.
+                exploit (WTYE); try eapply B; ss; auto; i; ss.
+              + erewrite <- alignof_blockcopy_wt_stable; eauto.
+                exploit (WTYE); try eapply B; ss; auto; i; ss.
+              + erewrite <- sizeof_wt_stable; eauto.
+                exploit (WTYE ty1); eauto. eapply B. ss. auto.
+              + erewrite <- sizeof_wt_stable; eauto.
+                exploit (WTYE ty1); eauto. eapply B. ss. auto. }
+        * econs 5; eauto.
+    - ss.
+      inversion STEP; subst; inv ST; ss; try (by eexists; right; econs; eauto).
+      + destruct k3; destruct k0; ss; clarify; try (by  eexists; right; econs; eauto).
+        inv SUM. unfold is_call_cont_strong in CALL. des_ifs.
+      + destruct k3; destruct k0; ss; clarify; try (by  eexists; right; econs; eauto).
+        inv SUM. unfold is_call_cont_strong in CALL. des_ifs.
+      + destruct k3; destruct k0; ss; clarify; try (by  eexists; right; econs; eauto).
+        inv SUM. unfold is_call_cont_strong in CALL. des_ifs.
+      + destruct k3; destruct k0; ss; clarify; try (by  eexists; right; econs; eauto).
+        inv SUM. unfold is_call_cont_strong in CALL. des_ifs.
+      + destruct k3; destruct k0; ss; clarify; try (by  eexists; right; econs; eauto).
+        inv SUM. unfold is_call_cont_strong in CALL. des_ifs.
+      + destruct k3; destruct k0; ss; clarify; try (by  eexists; right; econs; eauto).
+        inv SUM. unfold is_call_cont_strong in CALL. des_ifs.
+      + destruct k3; destruct k0; ss; clarify; try (by  eexists; right; econs; eauto).
+        inv SUM. unfold is_call_cont_strong in CALL. des_ifs.
+      + destruct k3; destruct k0; ss; clarify; try (by  eexists; right; econs; eauto).
+        inv SUM. unfold is_call_cont_strong in CALL. des_ifs.
+      + destruct k3; destruct k0; ss; clarify; try (by  eexists; right; econs; eauto).
+        inv SUM. unfold is_call_cont_strong in CALL. des_ifs.
+      + destruct k3; destruct k0; ss; clarify; try (by  eexists; right; econs; eauto).
+        inv SUM. unfold is_call_cont_strong in CALL. des_ifs.
+      + destruct k3; destruct k0; ss; clarify; try (by  eexists; right; econs; eauto).
+        inv SUM. unfold is_call_cont_strong in CALL. des_ifs.
+      + destruct k3; destruct k0; ss; clarify; try (by  eexists; right; econs; eauto).
+        inv SUM. unfold is_call_cont_strong in CALL. des_ifs.
+      + destruct k3; destruct k0; ss; clarify; try (by  eexists; right; econs; eauto).
+        inv SUM. unfold is_call_cont_strong in CALL. des_ifs.
+      + destruct k3; destruct k0; ss; clarify; try (by  eexists; right; econs; eauto).
+        inv SUM. unfold is_call_cont_strong in CALL. des_ifs.
+      + destruct k3; destruct k0; ss; clarify; try (by  eexists; right; econs; eauto).
+        inv SUM. unfold is_call_cont_strong in CALL. des_ifs.
+      + destruct k3; destruct k0; ss; clarify; try (by  eexists; right; econs; eauto).
+        inv SUM. unfold is_call_cont_strong in CALL. des_ifs.
+      + destruct k3; destruct k0; ss; clarify; try (by  eexists; right; econs; eauto).
+        inv SUM. unfold is_call_cont_strong in CALL. des_ifs.
+      + destruct k3; destruct k0; ss; clarify; try (by  eexists; right; econs; eauto).
+        inv SUM. unfold is_call_cont_strong in CALL. des_ifs.
+      + eexists. right.
+        ss. rpapply step_return_0; eauto.
+        inv WTTGT. exploit free_list_exists; eauto.
+      + destruct k3; destruct k0; ss; clarify; eauto;
+          inv SUM; unfold is_call_cont_strong in *; des_ifs.
+        * eexists. right.
+          ss. rpapply step_return_2; eauto.
+          inv WTTGT. exploit free_list_exists; eauto.
+        * eexists. right.
+          ss. rpapply step_return_2; eauto.
+          inv WTTGT. exploit free_list_exists; eauto.
+      + eexists. right. ss. eapply step_skip_call; eauto.
+        * exploit Cstrategy.is_call_cont_call_cont; et. intro T.
+          (* TODO: make lemma *)
+          clear - H T SUM. unfold is_call_cont in H. des_ifs. ss.
+          destruct k3; destruct k0; ss.
+          inv SUM; ss. des; clarify.
+          destruct k3; ss.
+          destruct k3; ss.
+        * inv WTTGT; ss.
+          exploit free_list_exists; eauto.
+      + destruct k3; destruct k0; ss; clarify; try (by eexists; right; econs; eauto).
+        inv SUM. unfold is_call_cont_strong in CALL. des_ifs.
+      + destruct k3; destruct k0; ss; clarify; try (by eexists; right; econs; eauto).
+        inv SUM. unfold is_call_cont_strong in CALL. des_ifs.
+      + destruct k3; destruct k0; ss; clarify; try (by eexists; right; econs; eauto).
+        inv SUM. unfold is_call_cont_strong in CALL. des_ifs.
+      + eexists. right. ss. eapply step_goto; et.
+        clear -H SUM.
+        erewrite <- call_cont_app_cont in H; et.
+        remember (fn_body f) as s. clear Heqs.
+        remember (call_cont k3) as k1. clear Heqk1.
+        admit "??".
+      + eexists. right.
+        destruct (lift_option (Genv.find_funct (SkEnv.revive (SkEnv.project skenv_link (CSk.of_program signature_of_function cp)) cp) fptr)) as [[gd TG] | TG].
+        { assert (gd = Internal f).
+          { unfold Genv.find_funct in *. des_ifs. rewrite Genv.find_funct_ptr_iff in *.
+            unfold Genv.find_def in *. ss.
+            do 2 rewrite MapsC.PTree_filter_map_spec, o_bind_ignore in *. des_ifs.
+            destruct (Genv.invert_symbol skenv_link b) eqn:SKENV; ss. unfold o_bind in Heq, Heq1. ss. des_ifs.
+            destruct (Genv.invert_symbol (SkEnv.project skenv_link (CSk.of_program signature_of_function cp_link)) b) eqn:LINKSYMB; ss.
+            destruct (Genv.invert_symbol (SkEnv.project skenv_link (CSk.of_program signature_of_function cp)) b) eqn:PROGSYMB; ss.
+            unfold o_bind in FPTR, TG. ss.
+            assert (i0 = i1) by admit "true".
+            assert (i = i1) by admit "true".
+            subst.
+            destruct ((prog_defmap cp_link) ! i1) eqn:DMAP; ss.
+            destruct ((prog_defmap cp) ! i1) eqn:DMAP0; ss. clarify.
+            rewrite CSk.of_program_internals in *.
+            unfold internals in Heq2. rewrite DMAP0 in Heq2. ss.
+            exploit prog_defmap_func_same_rev; eauto. i. Eq. auto. }
+          subst. inv WTTGT; ss.
+          eapply step_internal_function; eauto.
+          exploit preservation_alloc; eauto.
+          exploit preservation_bind_param; eauto.
+        }
+        { (* not call *)
+          exfalso.
+          eapply NCALLTGT.
+          (* destruct k3 eqn:Hk3; ss. *)
+          eexists.
+          econs; eauto.
+          - assert (Genv.find_funct skenv_link fptr = Some (AST.Internal (signature_of_function f))).
+            { assert (SkEnv.wf skenv_link).
+              { eapply SkEnv.load_skenv_wf.
+                eapply link_list_preserves_wf_sk; eauto. }
+              dup FPTR.
+              unfold Genv.find_funct in FPTR. des_ifs. rewrite Genv.find_funct_ptr_iff in *.
+              unfold Genv.find_def in FPTR. ss.
+              do 2 rewrite PTree_filter_map_spec, o_bind_ignore in *.
+              des_ifs.
+              rewrite Genv.find_funct_ptr_iff in *.
+              unfold Genv.find_def. ss.
+              exploit SkEnv.project_impl_spec. eapply INCL_LINKED. i.
+              inv H3.
+              destruct (Genv.invert_symbol skenv_link b) eqn:SKENV; ss.
+              unfold o_bind in Heq. ss. des_ifs.
+              assert (Genv.find_def (SkEnv.project skenv_link (CSk.of_program signature_of_function cp_link)) b = Some (Gfun (AST.Internal (signature_of_function f)))).
+              { unfold Genv.find_def. ss. rewrite PTree_filter_map_spec, o_bind_ignore. des_ifs.
+                rewrite SKENV. unfold o_bind. ss. des_ifs.
+                destruct ((prog_defmap (CSk.of_program signature_of_function cp_link)) ! i) eqn:DMAP; ss.
+                clarify.
+                destruct (Genv.invert_symbol (SkEnv.project skenv_link (CSk.of_program signature_of_function cp_link)) b) eqn:CPLINKSYMB; ss.
+                unfold o_bind in FPTR. ss.
+                destruct ((prog_defmap cp_link) ! i0) eqn:DMAP0; ss. clarify.
+                assert (i = i0) by admit "true". subst.
+                (* unfold CSk.of_program in DMAP. ss. unfold prog_defmap in DMAP, DMAP0. ss. *)
+                clear - DMAP DMAP0.
+                unfold prog_defmap in DMAP. ss.
+                unfold prog_defmap in DMAP0. ss.
+                unfold skdefs_of_gdefs in DMAP. ss.
+                do 2 rewrite prog_defmap_update_snd in DMAP.
+                rewrite DMAP0 in *. ss. }
+              exploit DEFKEPT; eauto. i. des.
+              inv LO. inv H6.  eauto. }
+              esplits; eauto. ss.
+              unfold signature_of_function. unfold signature_of_type. ss.
+              f_equal. remember (fn_params f) as l. clear Heql.
+              clear.
+              induction l. ss. ss.
+              destruct a. ss. rewrite IHl. eauto.
+          - inv WTTGT. ss.
+            inv WTK; ss.
+            exploit WTKS.
+            { ii. unfold fundef in *. Eq. }
+            i. des. clarify. }
+      + eexists. right.
+        destruct (lift_option (Genv.find_funct (SkEnv.revive (SkEnv.project skenv_link (CSk.of_program signature_of_function cp)) cp) fptr)) as [[gd TG] | TG].
+        {
+          assert (gd = (External ef targs tres cc)).
+          { unfold Genv.find_funct in *. des_ifs. rewrite Genv.find_funct_ptr_iff in *.
+            unfold Genv.find_def in *. ss.
+            do 2 rewrite MapsC.PTree_filter_map_spec, o_bind_ignore in *. des_ifs.
+            destruct (Genv.invert_symbol skenv_link b) eqn:SKENV; ss. unfold o_bind in Heq, Heq1. ss. des_ifs.
+            destruct (Genv.invert_symbol (SkEnv.project skenv_link (CSk.of_program signature_of_function cp_link)) b) eqn:LINKSYMB; ss.
+            destruct (Genv.invert_symbol (SkEnv.project skenv_link (CSk.of_program signature_of_function cp)) b) eqn:PROGSYMB; ss.
+            unfold o_bind in FPTR, TG. ss.
+            assert (i0 = i1) by admit "true".
+            assert (i = i1) by admit "true".
+            subst.
+            destruct ((prog_defmap cp_link) ! i1) eqn:DMAP; ss.
+            destruct ((prog_defmap cp) ! i1) eqn:DMAP0; ss. clarify.
+            rewrite CSk.of_program_internals in *.
+            unfold internals in Heq2. rewrite DMAP0 in Heq2. ss.
+            exploit prog_defmap_func_same_rev; eauto. i. Eq. auto. }
+          subst. eapply step_external_function; eauto. }
+        { (* not call *)
+          exfalso.
+          eapply NCALLTGT.
+          (* destruct k3 eqn:Hk3; ss. *)
+          eexists.
+          dup FPTR.
+          unfold Genv.find_funct in FPTR. des_ifs. rewrite Genv.find_funct_ptr_iff in *.
+          unfold Genv.find_def in FPTR. ss.
+          do 2 rewrite PTree_filter_map_spec, o_bind_ignore in *.
+          des_ifs.
+          rewrite Genv.find_funct_ptr_iff in *.
+          destruct (Genv.invert_symbol skenv_link b) eqn:SKENV; ss.
+          unfold o_bind in Heq. ss. des_ifs.
+          destruct ((prog_defmap (CSk.of_program signature_of_function cp_link)) ! i) eqn:DMAP; ss.
+          clarify.
+          destruct (Genv.invert_symbol (SkEnv.project skenv_link (CSk.of_program signature_of_function cp_link)) b) eqn:CPLINKSYMB; ss.
+          unfold o_bind in FPTR. ss.
+          destruct ((prog_defmap cp_link) ! i0) eqn:DMAP0; ss. clarify.
+          assert (i = i0) by admit "true". subst.
+          econs; eauto.
+          - assert (Genv.find_funct skenv_link (Vptr b Ptrofs.zero) = Some (AST.External ef)).
+            { assert (SkEnv.wf skenv_link).
+              { eapply SkEnv.load_skenv_wf.
+                eapply link_list_preserves_wf_sk; eauto. }
+              unfold Genv.find_def. ss.
+              exploit SkEnv.project_impl_spec. eapply INCL_LINKED. i.
+              inv H1.
+              assert (Genv.find_def (SkEnv.project skenv_link (CSk.of_program signature_of_function cp_link)) b = Some (Gfun (AST.External ef))).
+              { unfold Genv.find_def. ss. rewrite PTree_filter_map_spec, o_bind_ignore. des_ifs.
+                rewrite SKENV. unfold o_bind. ss. des_ifs.
+                (* unfold CSk.of_program in DMAP. ss. unfold prog_defmap in DMAP, DMAP0. ss. *)
+                clear - DMAP DMAP0. rewrite DMAP. ss.
+                unfold prog_defmap in DMAP. ss.
+                unfold prog_defmap in DMAP0. ss.
+                unfold skdefs_of_gdefs in DMAP. ss.
+                do 2 rewrite prog_defmap_update_snd in DMAP.
+                rewrite DMAP0 in *. ss. }
+              exploit DEFKEPT; eauto. i. des.
+              inv LO. inv H4; des_ifs; rewrite Genv.find_funct_ptr_iff; eauto. }
+            esplits; eauto.
+            inv WTPROGLINK.
+            unfold prog_defmap in DMAP0. ss. eapply PTree_Properties.in_of_list in DMAP0.
+            exploit H2; eauto.
+          - inv WTTGT. ss.
+            inv WTK; ss.
+            exploit WTKS.
+            { ii. unfold fundef in *. Eq. }
+            i. des. clarify. }
+      + destruct k3; destruct k0; ss; clarify; try (by eexists; right; econs; eauto).
+        inv SUM. unfold is_call_cont_strong in CALL. des_ifs.
+        ss. exfalso. eapply NRETTGT. ss. econs. unfold ModSem.final_frame. ss.
+        Unshelve. all:auto.
+  Qed.
 
 End SIM.
